fast/AvgFast.lean
@@ -1,3 +1,0 @@
-import AvgFast.Impl
-import AvgFast.Proofs
-import AvgFast.Naive
